BinaryHeap/CompleteTree/Lemmas.lean
@@ -29,6 +29,8 @@ theorem CompleteTree.rightLen_unfold {α : Type u} {o p : Nat} (v : α) (l : Com
 /-- Helper to rw away right, because Lean 4.9 makes it unnecessarily hard to deal with match in tactics mode... -/
 theorem CompleteTree.right_unfold {α : Type u} {o p : Nat} (v : α) (l : CompleteTree α o) (r : CompleteTree α p) (h₁ : p ≤ o) (h₂ : o < 2 * (p + 1)) (h₃ : (o + 1).isPowerOfTwo ∨ (p + 1).isPowerOfTwo) (h₄ : o + p + 1 > 0): (CompleteTree.branch v l r h₁ h₂ h₃).right h₄ = r := rfl
 
+theorem CompleteTree.contains_unfold {α : Type u} {o p : Nat} (element : α) (v : α) (l : CompleteTree α o) (r : CompleteTree α p) (h₁ : p ≤ o) (h₂ : o < 2 * (p + 1)) (h₃ : (o + 1).isPowerOfTwo ∨ (p + 1).isPowerOfTwo) : (CompleteTree.branch v l r h₁ h₂ h₃).contains element = (v=element ∨ l.contains element ∨ r.contains element) := rfl
+
 theorem CompleteTree.heqSameLeftLen {α : Type u} {n m : Nat} {a : CompleteTree α n} {b : CompleteTree α m} (h₁ : n = m) (h₂ : n > 0) (h₃ : HEq a b) : a.leftLen h₂ = b.leftLen (h₁.subst h₂) := by
   subst n
   have h₃ : a = b := eq_of_heq h₃
